LeanMqtt.lean
@@ -2,3 +2,5 @@
 -- Import modules here that should be built as part of the library.
 import LeanMqtt.Packets.Basic
 import LeanMqtt.Packets.Proofs
+import LeanMqtt.Packets.ReasonCode.Basic
+import LeanMqtt.Packets.ReasonCode.Proofs
