LeanMqtt/Packets/ReasonCode/Proofs.lean
@@ -1,0 +1,41 @@
+import LeanMqtt.Primitives.UInt.Proofs
+import LeanMqtt.Packets.ReasonCode.Basic
+import LeanMqtt.Helpers.ParserTactics
+
+namespace Mqtt
+
+theorem ReasonCode.byte_roundtrip (rc : ReasonCode) :
+    ReasonCode.decode? (ReasonCode.encode rc) = some rc := by
+  cases rc <;> rfl
+
+theorem ReasonCode.byte_reconstruct {rc : ReasonCode} {b : UInt8} :
+    ReasonCode.decode? b = some rc → ReasonCode.encode rc = b := by
+  unfold decode? encode
+  split
+  all_goals {
+    intro h
+    cases h
+    try rfl
+  }
+
+theorem ReasonCode.roundtrip (rc : ReasonCode) {rest : List UInt8} :
+    ReasonCode.parser.run (rc.serialize ++ rest) = some (rc, rest) := by
+  simp [ReasonCode.parser, ReasonCode.serialize, ReasonCode.encode, ReasonCode.decode?]
+  cases rc <;> rfl
+
+theorem ReasonCode.reconstruct {rc : ReasonCode} {input rest : List UInt8} :
+    ReasonCode.parser.run input = some (rc, rest) → input = rc.serialize ++ rest := by
+  simp only [ReasonCode.parser, ReasonCode.serialize]
+  intro h
+
+  step_parser h → bVal rest1 h_bVal
+
+  finish_parser h → h_rcOpt
+
+  rw [UInt8.reconstruct h_bVal]
+
+  have h_byte_eq := ReasonCode.byte_reconstruct h_rcOpt
+  rw [← h_byte_eq]
+  rfl
+
+end Mqtt
